Test/linear/README.dfy
@@ -1,0 +1,365 @@
+// RUN: %dafny /compile:0 /print:"%t.print" /dprint:"%t.dprint" /autoTriggers:0 "%s" > "%t"
+// RUN: %diff "%s.expect" "%t"
+
+/*
+This file describes an experimental "linearity" extension to Dafny.
+With this extension, Dafny programs can declare "linear variables",
+which cannot be duplicated and cannot be discarded.
+This allows programs to express in-place updates of functional data structures.
+It also allows manual memory management of functional data structures.
+
+Each Dafny variable is one of the following:
+  - "ghost"
+  - "linear"
+  - "shared"
+  - ordinary (no annotation)
+For example:
+    ghost var xg:T;
+    linear var xl:T;
+    shared var xs:T;
+    var xo:T;
+
+Ghost, linear, shared, and ordinary variables may be assigned to ghost variables:
+    xg := xg';
+    xg := xl';
+    xg := xs';
+    xg := xo';
+Linear variables may be assigned to linear variables:
+    xl := xl';
+Shared variables may be assigned to shared variables:
+    xs := xs';
+Ordinary variables may be assigned to ordinary variables:
+    xo := xo';
+Other assignments are disallowed
+(except for a special case of "borrowing" linear variables into shared variables, described below).
+*/
+
+method Vars<T>(ghost xg_in:T, linear xl_in:T, shared xs_in:T, xo_in:T) returns(linear xl_out:T)
+{
+    ghost var xg:T;
+    linear var xl:T;
+    shared var xs:T;
+    var xo:T;
+
+    xg := xg_in;
+    xg := xl_in;
+    xg := xs_in;
+    xg := xo_in;
+    xl := xl_in;
+    xs := xs_in;
+    xo := xo_in;
+
+    xl_out := xl;
+}
+
+/*
+Linear variables cannot be duplicated.
+The following is disallowed because it tries to duplicate xl:
+  linear var xl := ...;
+  linear var xl1 := xl;
+  linear var xl2 := xl;
+Linear variables cannot be discarded.
+The following is disallowed because it tries to discard xl at the end of a block:
+  {
+    linear var xl := ...;
+    // xl discarded at end of block
+  }
+At any place in a program, a linear variable is either "available" or "unavailable".
+When a linear variable is assigned, it becomes available.
+When a linear variable is used, it becomes unavailable (it is "consumed" by the use).
+It is illegal to use an unavailable variable; this prevents duplication.
+It is illegal to let an available variable go out of scope; this prevents discarding.
+For example:
+  linear var xl := ...;
+  // xl is available
+  linear var xl1 := xl; // ok, because xl is available here
+  // xl is unavailable, xl1 is available
+  linear var xl2 := xl; // illegal: tries to use xl, which is unavailable here 
+Notice that the "Vars" method shown above returns a linear result "xl_out".
+This is because it can't simply let xl go out of scope while it is still available;
+it must assign xl to some other variable, like xl_out.
+Furthermore, any linear return values like xl_out must be available at method exit.
+Any linear input parameters like xl_in are assumed to be available at method entry.
+*/
+
+/*
+Datatypes may be declared linear:
+*/
+linear datatype ld = LD(i:int)
+
+/*
+A constructor of a linear datatype produces a linear value that can be stored in a linear variable:
+*/
+method Test_ld_1() returns(linear x:ld)
+{
+    x := LD(10);
+}
+
+/*
+Linear datatypes are deconstructed with linear pattern matching
+(or with shared pattern matching, described later):
+*/
+method Test_ld_2(b:bool, linear x:ld)
+{
+    if (b)
+    {
+        linear match x {case LD(i) => print i + i;}
+    }
+    else
+    {
+        // Alternate syntax for linear match when there's only one case:
+        linear var LD(i) := x;
+        print i + i;
+    }
+}
+
+/*
+Linear datatypes may contain linear fields, which store linear values:
+*/
+linear datatype lOption<A> = LNone | LSome(linear a:A)
+linear datatype nlPair<A, B> = NlPair(a:A, linear b:B)
+linear datatype llPair<A, B> = LlPair(linear a:A, linear b:B)
+linear datatype nlList<A> = NlNil | NlCons(hd:A, linear tl:nlList<A>)
+
+function method IncrAll(linear l:nlList<int>):linear nlList<int>
+{
+    linear match l
+    {
+        case NlNil => NlNil
+        case NlCons(hd, tl) => NlCons(hd + 1, IncrAll(tl))
+    }
+}
+
+/*
+It is often convenient to temporarily duplicate a linear variable when reading it.
+This is supported by "shared" variables, which may temporarily "borrow" a linear variable
+for read-only operations.
+For example, the Length function below reads a linear list to compute its length.
+*/
+
+function method Length<A>(shared s:nlList<A>):int
+{
+    shared match s
+    {
+        case NlNil => 0
+        case NlCons(_, tl) => 1 + Length(tl)
+    }
+}
+
+function method MakeEven(linear l:nlList<int>):linear nlList<int>
+{
+    var len:int := Length(l); // borrow linear l into shared s when calling Length
+    if len % 2 == 0 then l else NlCons(0, l)
+}
+
+/*
+A variable binding expression like "var x := e1; e2" may freely borrow a linear variable x inside e1
+as long as it eventually consumes x in e2.
+Note that borrowing must strictly precede consumption;
+it would be illegal, for example, for "var x := e1; e2" to consume x in e1
+and then try to borrow it in e2.
+It would also be illegal to consume x and borrow x side by side,
+since expression evaluation order is underspecified:
+  f(Length(l), IncrAll(l)) // not allowed -- IncrAll could deallocate l before Length reads it, depending on the compiler
+To work around this limitation, simply use a temporary variable:
+  var len := Length(l);
+  f(len, IncrAll(l)) // ok
+
+Here are some additional examples of sharing:
+*/
+
+function method Share2(linear l:nlList<int>):linear nlList<int>
+{
+    var w:int := Length(l) + Length(l);
+    var x:int := if l.NlNil? then 0 else l.hd + l.hd;
+    var y:int := (
+        shared var s := l;
+        shared var s1 := s;
+        shared var s2 := s;
+        Length(s1) + Length(s2)
+    );
+    var z:int := (
+        shared match l
+        {
+            case NlNil => 0
+            case NlCons(sa, sb) => sa + Length(sb)
+        }
+    );
+    NlCons(w + x + y + z, l)
+}
+
+/*
+Unfortunately, it is not yet possible for statements to
+directly borrow a linear variable into a shared variable:
+  method M(linear l:nlList<int>)
+  {
+      {
+          shared var s := l; // would be useful, but is not yet supported
+          ...use s...
+      }
+      ...use l...
+  }
+
+Instead, a method can indirectly borrow by calling another method,
+as in the example below.
+(Important restriction: if a method call borrows a linear argument into
+a shared parameter, the method is not allowed to return a shared result.
+This prevents the method from trying to return the original linear value
+back to the caller as a (duplicated) shared value.)
+*/
+
+method Inner<A>(shared s_in:nlList<A>) returns(len:int)
+    ensures len == Length(s_in)
+{
+    shared var s := s_in;
+    len := 0;
+    while (s.NlCons?)
+        invariant Length(s) + len == Length(s_in)
+        decreases s
+    {
+        len := len + 1;
+        s := s.tl;
+    }
+}
+
+method Outer(linear l_in:nlList<int>) returns(linear l:nlList<int>)
+{
+    l := l_in;
+    var len := Inner(l); // ok: borrow l by calling Inner
+    var doubleLen := Length(l) + Length(l); // ok: borrow l inside expression
+    assert doubleLen == len * 2;
+}
+
+/*
+In-place updates to sequences are a useful application of linearity.
+We can define linear operations on seq<A>, which contains ordinary values,
+and on lseq<A>, which contains linear values.
+
+Notice that seq supports get and set, while lseq only supports swap.
+This is because get and set duplicate and discard, which is not allowed on linear values,
+whereas swap simply exchanges one linear value for another, which is allowed.
+
+To help with swapping, the maybe<A> type optionally holds an A value,
+depending on whether the ghost property has(m) is true or false.
+Get and set operations for lseq swap a maybe<A> value with has(m) == true for
+a maybe<A> value with has(m) == false.
+*/
+
+function method seq_get<A>(shared s:seq<A>, i:nat):(a:A)
+    requires i < |s|
+    ensures a == s[i]
+function method seq_set<A>(linear s1:seq<A>, i:nat, a:A):(linear s2:seq<A>) // can be implemented as in-place update
+    requires i < |s1|
+    ensures s2 == s1[i := a]
+function method seq_length<A>(shared s:seq<A>):(n:nat)
+    ensures n == |s|
+
+method seq_alloc<A>(length:nat) returns(linear s:seq<A>)
+    ensures |s| == length
+
+method seq_free<A>(linear s:seq<A>)
+
+type maybe<A>
+predicate has<A>(m:maybe<A>)
+function read<A>(m:maybe<A>):A
+function method peek<A>(shared m:maybe<A>):(shared a:A)
+    requires has(m)
+    ensures a == read(m)
+function method take<A>(linear m:maybe<A>):(linear a:A)
+    requires has(m)
+    ensures a == read(m)
+function method give<A>(linear a:A):(linear m:maybe<A>)
+    ensures has(m)
+    ensures read(m) == a
+    ensures forall x:maybe<A> {:trigger give(read(x))} | has(x) && a == read(x) :: m == x
+function method empty<A>():(linear m:maybe<A>)
+    ensures !has(m)
+function method discard<A>(linear m:maybe<A>):()
+    requires !has(m)
+
+type lseq<A>
+function lseqs<A>(s:lseq<A>):seq<maybe<A>> // contents of an lseq, as ghost seq
+function method lseq_length<A>(shared s:lseq<A>):(n:nat)
+    ensures n == |lseqs(s)|
+
+method lseq_alloc<A>(length:nat) returns(linear s:lseq<A>)
+    ensures |lseqs(s)| == length
+    ensures forall i:nat | i < length :: !has(lseqs(s)[i])
+
+method lseq_free<A>(linear s:lseq<A>)
+    requires forall i:nat | i < |lseqs(s)| :: !has(lseqs(s)[i])
+
+// can be implemented as in-place swap
+method lseq_swap<A>(linear s1:lseq<A>, i:nat, linear a1:maybe<A>) returns(linear s2:lseq<A>, linear a2:maybe<A>)
+    requires i < |lseqs(s1)|
+    ensures a2 == lseqs(s1)[i]
+    ensures lseqs(s2) == lseqs(s1)[i := a1]
+
+function method lseq_share<A>(shared s:lseq<A>, i:nat):(shared a:maybe<A>)
+    requires i < |lseqs(s)|
+    ensures a == lseqs(s)[i]
+
+function method lseq_peek<A>(shared s:lseq<A>, i:nat):(shared a:A)
+    requires i < |lseqs(s)|
+    requires has(lseqs(s)[i])
+    ensures a == peek(lseqs(s)[i])
+{
+    peek(lseq_share(s, i))
+}
+
+method lseq_get<A>(linear s1:lseq<A>, i:nat) returns(linear s2:lseq<A>, linear a:A)
+    requires i < |lseqs(s1)|
+    requires has(lseqs(s1)[i])
+    ensures a == read(lseqs(s1)[i])
+    ensures lseqs(s2) == lseqs(s1)[i := empty()]
+{
+    linear var x1:maybe<A> := empty();
+    linear var x2:maybe<A>;
+    s2, x2 := lseq_swap(s1, i, x1);
+    a := take(x2);
+}
+
+method lseq_set<A>(linear s1:lseq<A>, i:nat, linear a:A) returns(linear s2:lseq<A>)
+    requires i < |lseqs(s1)|
+    requires !has(lseqs(s1)[i])
+    ensures lseqs(s2) == lseqs(s1)[i := give(a)]
+{
+    linear var x1:maybe<A> := give(a);
+    linear var x2:maybe<A>;
+    s2, x2 := lseq_swap(s1, i, x1);
+    var _ := discard(x2);
+}
+
+method SeqExample<A>(linear s_in:lseq<nlList<A>>) returns(linear s:lseq<nlList<A>>, linear lens:seq<int>)
+    requires forall i:nat | i < |lseqs(s_in)| :: has(lseqs(s_in)[i])
+    ensures lseqs(s) == lseqs(s_in)
+    ensures |lens| == |lseqs(s)|
+    ensures forall i:nat | i < |lens| :: lens[i] == Length(read(lseqs(s)[i]))
+{
+    // Compute length of every list in s_in
+    s := s_in;
+    var len := lseq_length(s);
+    lens := seq_alloc(len);
+    var i:nat := 0;
+    while (i < len)
+        invariant i <= len
+        invariant lseqs(s) == lseqs(s_in)
+        invariant |lens| == len
+        invariant forall j:nat | j < i :: lens[j] == Length(read(lseqs(s)[j]))
+    {
+        if (*)
+        {
+            // The hard way to do it:
+            linear var l:nlList<A>;
+            s, l := lseq_get(s, i);
+            lens := seq_set(lens, i, Length(l));
+            s := lseq_set(s, i, l);
+        }
+        else
+        {
+            // The easy way to do it:
+            lens := seq_set(lens, i, Length(lseq_peek(s, i)));
+        }
+        i := i + 1;
+    }
+}
